<?xml version="1.0" encoding="UTF-8"?>
<!-- 
    WARNING:  THIS IS A WORKING DRAFT ONTOLOGY AND STILL UNDER DEVELOPMENT, this file will change frequently and significantly as development continues.
    
    Note:  http://measurement.bibliotek-o.org/ is a placeholder (fake) namespace for the LD4P/L Measurements ontology extension until a proper home is found
  -->

<rdf:RDF xmlns="http://measurement.bibliotek-o.org/"
    xmlns:bf="http://id.loc.gov/ontologies/bibframe/" xmlns:bib="http://bibliotek-o.org/ontology/"
    xmlns:dcterms="http://purl.org/dc/terms/" xmlns:owl="http://www.w3.org/2002/07/owl#"
    xmlns:rdf="http://www.w3.org/1999/02/22-rdf-syntax-ns#"
    xmlns:rdfs="http://www.w3.org/2000/01/rdf-schema#"
    xmlns:skos="http://www.w3.org/2004/02/skos/core#" xmlns:xsd="http://www.w3.org/2001/XMLSchema#"
    xmlns:foaf="http://xmlns.com/foaf/0.1#" xmlns:vann="http://purl.org/vocab/vann/"
    xmlns:voaf="http://purl.org/vocommons/voaf#">

    <!-- ONTOLOGY DECLARATION -->

    <owl:Ontology rdf:about="http://measurement.bibliotek-o.org/">
        <owl:versionInfo rdf:datatype="http://www.w3.org/2001/XMLSchema#string">Version
            0.0</owl:versionInfo>
        <rdfs:label xml:lang="en">ArtFrame: extension ontology for describing art
            materials</rdfs:label>
        <vann:preferredNamespacePrefix>meas</vann:preferredNamespacePrefix>
        <rdfs:comment xml:lang="en">This measurements ontology was developed as a stand alone
            ontology as part of the bibliotek-o BIBFRAME 2.0 extension ontology
            project</rdfs:comment>
        <voaf:extends rdf:resource="http://bibliotek-o.org/ontology/"/>
        <voaf:specializes rdf:resource="http://bibliotek-o.org/ontology/"/>
    </owl:Ontology>


    <!-- CLASSES -->

    <owl:Class rdf:about="http://measurement.bibliotek-o.org/MeasurementGroup">
        <rdfs:label>Measurement Group</rdfs:label>
        <skos:definition xml:lang="en-us">A set of measurements pertaining to a specific resource,
            part of a resource, or resource in a particular arrangement. For example, a book may
            have a specified height, width, length, and/or weight, which are all attached to a
            MeasurementGroup; the binding may have measurements specified independently, which would
            constitute another MeasurementGroup. A MeasurementGroup has one or more specific
            Measurements attached to it.</skos:definition>
    </owl:Class>

    <owl:Class rdf:about="http://measurement.bibliotek-o.org/Measurement">
        <rdfs:label>Measurement</rdfs:label>
        <skos:definition xml:lang="en-us">The measurement of a single aspect of a resource,
            including value, units, and the dimension measured. For example, a book may have a
            height (aspect) of 10 (value) centimeters (units). Each such measurement is attached to
            a MeasurementGroup.</skos:definition>
    </owl:Class>

    <owl:Class rdf:about="http://measurement.bibliotek-o.org/Arrangement">
        <rdfs:label>Arrangement</rdfs:label>
        <skos:definition xml:lang="en-us">The arrangement, organization, or configuration of a
            single object or collection of objects. For example, a parchment may be rolled or
            unrolled; a collection of visual materials has a specific arrangement; computer files
            are organized and ordered in a specific way.</skos:definition>
    </owl:Class>

    <!-- OBJECT PROPERTIES -->

    <owl:ObjectProperty rdf:about="http://measurement.bibliotek-o.org/hasMeasurementGroup">
        <rdfs:label xml:lang="en">has measurement group</rdfs:label>
        <skos:definition xml:lang="en">The relationship of a resource to a measurement group,
            indicating that the measurement group applies to the resource.</skos:definition>
        <rdfs:range rdf:resource="http://measurement.bibliotek-o.org/MeasurementGroup"/>
        <owl:inverseOf rdf:resource="http://measurement.bibliotek-o.org/isMeasurementGroupOf"/>
    </owl:ObjectProperty>

    <owl:ObjectProperty rdf:about="http://measurement.bibliotek-o.org/isMeasurementGroupOf">
        <rdfs:label xml:lang="en">is measurement group of</rdfs:label>
        <skos:definition xml:lang="en">The relationship of a measurement group to a resource,
            indicating that the measurement group applies to the resource.</skos:definition>
        <rdfs:domain rdf:resource="http://measurement.bibliotek-o.org/MeasurementGroup"/>
        <owl:inverseOf rdf:resource="http://measurement.bibliotek-o.org/hasMeasurementGroup"/>
    </owl:ObjectProperty>

    <owl:ObjectProperty rdf:about="http://measurement.bibliotek-o.org/hasMeasurement">
        <rdfs:label xml:lang="en">has measurement</rdfs:label>
        <skos:definition xml:lang="en">The relationship of a reasourse to a
            measurement.</skos:definition>
        <rdfs:range rdf:resource="http://measurement.bibliotek-o.org/Measurement"/>
        <owl:inverseOf rdf:resource="http://measurement.bibliotek-o.org/isMeasurementOf"/>
    </owl:ObjectProperty>

    <owl:ObjectProperty rdf:about="http://measurement.bibliotek-o.org/isMeasurementOf">
        <rdfs:label xml:lang="en">is measurement of</rdfs:label>
        <skos:definition xml:lang="en">The relationship of a measurement to a
            resource.</skos:definition>
        <rdfs:domain rdf:resource="http://measurement.bibliotek-o.org/Measurement"/>
        <owl:inverseOf rdf:resource="http://measurement.bibliotek-o.org/hasMeasurement"/>
    </owl:ObjectProperty>

    <owl:ObjectProperty rdf:about="http://measurement.bibliotek-o.org/measures">
        <rdfs:label xml:lang="en">measures</rdfs:label>
        <skos:definition xml:lang="en">The relationship between a Measurement and the dimension or
            other aspect of a resource that is measured by this Measurement. For example, a
            Measurement may specify the length, height, weight, file size, etc. of a
            resource.</skos:definition>
        <rdfs:domain rdf:resource="http://measurement.bibliotek-o.org/Measurement"/>
        <owl:inverseOf rdf:resource="http://measurement.bibliotek-o.org/measuredBy"/>
    </owl:ObjectProperty>

    <owl:ObjectProperty rdf:about="http://measurement.bibliotek-o.org/measuredBy">
        <rdfs:label xml:lang="en">measured by</rdfs:label>
        <skos:definition xml:lang="en">The relationship between a dimension or other aspect of a
            resource and the Measurement that measures it. For example, the length, height, weight,
            file size, etc. of a resource may be the aspect that is measured by a particular
            Measurement.</skos:definition>
        <rdfs:range rdf:resource="http://measurement.bibliotek-o.org/Measurement"/>
        <owl:inverseOf rdf:resource="http://measurement.bibliotek-o.org/measures"/>
    </owl:ObjectProperty>

    <owl:ObjectProperty rdf:about="http://measurement.bibliotek-o.org/hasUnit">
        <rdfs:label xml:lang="en">has unit</rdfs:label>
        <skos:definition xml:lang="en">Relationship between the measurement and the unit used to
            express the measurement.</skos:definition>
        <owl:inverseOf rdf:resource="http://measurement.bibliotek-o.org/isUnitOf"/>
    </owl:ObjectProperty>

    <owl:ObjectProperty rdf:about="http://measurement.bibliotek-o.org/isUnitOf">
        <rdfs:label xml:lang="en">is unit of</rdfs:label>
        <skos:definition xml:lang="en">Relationship between the unit and the measurement used to
            express the measurement.</skos:definition>
        <owl:inverseOf rdf:resource="http://measurement.bibliotek-o.org/hasUnit"/>
    </owl:ObjectProperty>

    <owl:ObjectProperty rdf:about="http://measurement.bibliotek-o.org/hasArrangement">
        <rdfs:label xml:lang="en">has arrangement</rdfs:label>
        <skos:definition xml:lang="en">Relationship between the resource and a specified
            arrangement, organization, or configuration of it.</skos:definition>
        <rdfs:range rdf:resource="http://measurement.bibliotek-o.org/Arrangement"/>
        <owl:inverseOf rdf:resource="http://measurement.bibliotek-o.org/isArrangementOf"/>
    </owl:ObjectProperty>

    <owl:ObjectProperty rdf:about="http://measurement.bibliotek-o.org/isArrangementOf">
        <rdfs:label xml:lang="en">is arrangement of</rdfs:label>
        <skos:definition xml:lang="en">Relationship between a specified arrangement, organization,
            or configuration and a resource.</skos:definition>
        <rdfs:domain rdf:resource="http://measurement.bibliotek-o.org/Arrangement"/>
        <owl:inverseOf rdf:resource="http://measurement.bibliotek-o.org/hasArrangement"/>
    </owl:ObjectProperty>

</rdf:RDF>
